change stuck definition to require reachability via the path condition

Pom/Lpo/Operations/Seq/Branches.lean
@@ -10,48 +10,52 @@ def ReachableWith (α : Lpofin (Label act test)) (φ : PathCond α) (x : Node) :
     ψ.toForm ≤ α.form x
 
 def Reachable (α : Lpofin (Label act test)) : Node → Prop :=
-  α.ReachableWith PathCond.empty
+  α.ReachableWith ⊥
 
-lemma reachable_isotone [Preorder act] [Preorder test] {α β : Lpofin (Label act test)} (hle : α ≤ β)
-    {x : Node} (hx : x ∈ α.nodes) : α.Reachable x ↔ β.Reachable x := by
+lemma reachable_isotone [Preorder act] [Preorder test] {α β : Lpofin (Label act test)}
+    {φ : PathCond α} (hle : α ≤ β)
+    {x : Node} (hx : x ∈ α.nodes) :
+    α.ReachableWith φ x ↔ β.ReachableWith (φ.up_cast hle) x := by
   constructor
-  · rintro ⟨ψ, _, hform⟩
-    refine ⟨ψ.up_cast hle, bot_le, ?_⟩; exact hform.trans (le_form hle)
-  · rintro ⟨ψ, _, hform⟩
+  · rintro ⟨ψ, hext, hform⟩
+    refine ⟨ψ.up_cast hle, hext, ?_⟩; exact hform.trans (le_form hle)
+  · rintro ⟨ψ, hext, hform⟩
     let ψ' : PathCond α := {
       tests := ψ.tests ∩ α.tests
       truth := fun ⟨z, hz⟩ ↦ ψ.truth ⟨z, Set.inter_subset_left hz⟩
       tests_valid := Set.inter_subset_right
     }
-    refine ⟨ψ', bot_le, ?_⟩
-    rw [← PathCond.cast_toForm (hle := hle)]; conv => rhs; exact hle.form x hx
-    refine PathCond.implies_weaken ?_ hform ?_
-    · refine ⟨Set.inter_subset_left, fun _ ↦ rfl⟩
-    · conv => arg 1; exact (hle.form x hx).symm
-      refine (α.val.property.form _ hx).1.monotone _ ?_
-      intro y hyx ⟨hyt, h⟩; refine h ⟨hyt, ?_⟩
-      obtain ⟨b, hb⟩ := (Label.isTest_iff _).mp (ψ.tests_valid hyt)
-      have hlab := le_of_le_of_eq (hle.lab y) hb
-      cases hy : α.lab y with
-      | bot => exfalso; exact α.val.property.bot y hy x hyx
-      | fork => have := le_of_eq_of_le hy.symm hlab; contradiction
-      | act a => have := le_of_eq_of_le hy.symm hlab; contradiction
-      | test t => exact (Label.isTest_iff _).mpr ⟨t, hy⟩
+    refine ⟨ψ', ⟨?_, ?_⟩, ?_⟩
+    · exact Set.subset_inter hext.1 φ.tests_valid
+    · intro x; exact hext.2 x
+    · rw [← PathCond.cast_toForm (hle := hle)]; conv => rhs; exact hle.form x hx
+      refine PathCond.implies_weaken ?_ hform ?_
+      · refine ⟨Set.inter_subset_left, fun _ ↦ rfl⟩
+      · conv => arg 1; exact (hle.form x hx).symm
+        refine (α.val.property.form _ hx).1.monotone _ ?_
+        intro y hyx ⟨hyt, h⟩; refine h ⟨hyt, ?_⟩
+        obtain ⟨b, hb⟩ := (Label.isTest_iff _).mp (ψ.tests_valid hyt)
+        have hlab := le_of_le_of_eq (hle.lab y) hb
+        cases hy : α.lab y with
+        | bot => exfalso; exact α.val.property.bot y hy x hyx
+        | fork => have := le_of_eq_of_le hy.symm hlab; contradiction
+        | act a => have := le_of_eq_of_le hy.symm hlab; contradiction
+        | test t => exact (Label.isTest_iff _).mpr ⟨t, hy⟩
 
-def reachable_pred {α : Lpofin (Label act test)} {x z : Node}
-    (hr : α.Reachable x) (hz : α.rel z x) : α.Reachable z := by
-  rcases hr with ⟨ψ, _, hform⟩
-  refine ⟨ψ, bot_le, ?_⟩
+def reachable_pred {α : Lpofin (Label act test)} {x z : Node} {φ : PathCond α}
+    (hr : α.ReachableWith φ x) (hz : α.rel z x) : α.ReachableWith φ z := by
+  rcases hr with ⟨ψ, hext, hform⟩
+  refine ⟨ψ, hext, ?_⟩
   exact hform.trans ((α.val.property.form z (α.val.property.rel_dom hz).1).2 x hz)
 
 -- stuck is a path condition formula indicating that the execution will definitely
 -- encounter a ⊥ node
-def stuck (α : Lpofin (Label act test)) : Form Node :=
-  Form.sOr fun x : ↑{ x ∈ α.nodes | α.lab x = ⊥ ∧ α.Reachable x } ↦ α.form x.val
+def stuck (α : Lpofin (Label act test)) (φ : PathCond α) : Form Node :=
+  Form.sOr fun x : ↑{ x ∈ α.nodes | α.lab x = ⊥ ∧ α.ReachableWith φ x } ↦ α.form x.val
 
-lemma stuck_antitone [PartialOrder act] [PartialOrder test] :
-    @Antitone (Lpofin (Label act test)) _ _ _ stuck := by
-  intro α β hle v ⟨⟨x, hx, hlab, hr⟩, hform⟩
+lemma stuck_antitone [PartialOrder act] [PartialOrder test] {α β : Lpofin (Label act test)}
+    {φ : PathCond α} (hle : α ≤ β) : β.stuck (φ.up_cast hle) ≤ α.stuck φ := by
+  intro v ⟨⟨x, hx, hlab, hr⟩, hform⟩
   rcases hle.succ _ hx with hx' | ⟨y, ⟨hy, hlab'⟩, hyx⟩
   · refine ⟨⟨x, hx', ?_, ?_⟩, ?_⟩
     · refine le_antisymm ?_ bot_le
@@ -72,9 +76,9 @@ def conj (α : Lpofin (Label act test)) (S : Set Node) : Form Node :=
 def branches (α : Lpofin (Label act test)) : Set (PathCond α) :=
   { φ : PathCond α
   | (∀ x ∈ φ.tests, φ.toForm ≤ α.form x) ∧
-    φ.toForm ≤ α.stuck.not ∧
+    φ.toForm ≤ (α.stuck φ).not ∧
     ∀ {x}, x ∉ φ.tests → α.isTest x →
-      ¬ (α.form x ≤ α.stuck) → ¬ α.ReachableWith φ x
+      ¬ (α.form x ≤ α.stuck φ) → ¬ α.ReachableWith φ x
   }
 
 lemma branches_finite (α : Lpofin (Label act test)) : α.branches.Finite := Set.toFinite _
@@ -130,23 +134,12 @@ lemma reachableWith_isotone [Preorder act] [Preorder test]
 
 lemma not_reachableWith_of_form_le_stuck
     {α : Lpofin (Label act test)} {φ : PathCond α} {x : Node}
-    (havoid : φ.toForm ≤ α.stuck.not) (hform : α.form x ≤ α.stuck) :
+    (havoid : φ.toForm ≤ (α.stuck φ).not) (hform : α.form x ≤ α.stuck φ) :
     ¬ α.ReachableWith φ x := by
   rintro ⟨η, hext, hη⟩
   rcases η.sat with ⟨v, hv⟩
   have hφv := PathCond.toForm_antitone hext v hv
   exact (havoid v hφv) (hform v (hη v hv))
-
-lemma reachable_of_reachableWith {α : Lpofin (Label act test)} {φ : PathCond α} {x : Node}
-    (hr : α.ReachableWith φ x) : α.Reachable x := by
-  rcases hr with ⟨ψ, _, hform⟩
-  exact ⟨ψ, bot_le, hform⟩
-
-lemma reachableWith_pred {α : Lpofin (Label act test)} {φ : PathCond α} {x z : Node}
-    (hr : α.ReachableWith φ x) (hz : α.rel z x) : α.ReachableWith φ z := by
-  rcases hr with ⟨ψ, hext, hform⟩
-  refine ⟨ψ, hext, ?_⟩
-  exact hform.trans ((α.val.property.form z (α.val.property.rel_dom hz).1).2 x hz)
 
 lemma branches_monotone [PartialOrder act] [PartialOrder test]
     {α β : Lpofin (Label act test)} (hle : α ≤ β)
@@ -164,26 +157,25 @@ lemma branches_monotone [PartialOrder act] [PartialOrder test]
     rcases isTest_of_le_or_bot hle htest with htestα | hbot
     · have hxα : x ∈ α.nodes := tests_sub_nodes htestα
       have hreachα := (reachableWith_isotone hle hxα).mpr hreach
-      by_cases hαstuck : α.form x ≤ α.stuck
+      by_cases hαstuck : α.form x ≤ α.stuck φ
       · exact not_reachableWith_of_form_le_stuck hstuck hαstuck hreachα
       · exact hmax hx htestα hαstuck hreachα
     · rcases hle.succ x hxβ with hxα | ⟨y, ⟨hyα, hybot⟩, hyx⟩
       · have hreachα := (reachableWith_isotone hle hxα).mpr hreach
         apply not_reachableWith_of_form_le_stuck hstuck _ hreachα
         intro v hxform
-        refine ⟨⟨x, hxα, hbot, ?_⟩, hxform⟩
-        exact reachable_of_reachableWith hreachα
+        exact ⟨⟨x, hxα, hbot, hreachα⟩, hxform⟩
       · have hreachyβ : β.ReachableWith (φ.up_cast hle) y :=
-          reachableWith_pred hreach hyx
+          reachable_pred hreach hyx
         have hreachy : α.ReachableWith φ y :=
           (reachableWith_isotone hle hyα).mpr hreachyβ
         apply not_reachableWith_of_form_le_stuck hstuck _ hreachy
         intro v hyform
-        refine ⟨⟨y, hyα, hybot, reachable_of_reachableWith hreachy⟩, hyform⟩
+        refine ⟨⟨y, hyα, hybot, hreachy⟩, hyform⟩
 
 lemma le_branches [PartialOrder act] [PartialOrder test] {α β : Lpofin (Label act test)}
     (hle : α ≤ β) : α.branches =
-      { φ | ∃ φ' ∈ β.branches, φ' = φ.up_cast hle ∧ φ.toForm ≤ α.stuck.not } := by
+      { φ | ∃ φ' ∈ β.branches, φ' = φ.up_cast hle ∧ φ.toForm ≤ (α.stuck φ).not } := by
   ext φ
   constructor
   · intro hφ
@@ -227,17 +219,20 @@ lemma branch_tests_subset_of_common_sat {α : Lpofin (Label act test)}
   intro x hx
   by_contra hnx
   have htest : α.isTest x := φ.tests_valid hx
-  have hnstuck : ¬ (α.form x ≤ α.stuck) := by
+  have hnstuck : ¬ (α.form x ≤ α.stuck φ) := by
     intro hle
     exact (hφ.2.1 v hsatφ) (hle v (hφ.1 x hx v hsatφ))
-  apply hψ.2.2 hnx htest hnstuck
   let η := ψ.union φ
   have hcompat {z} (hz : z ∈ ψ.tests ∩ φ.tests) :
       ψ.truth ⟨z, hz.1⟩ = φ.truth ⟨z, hz.2⟩ := by
     apply Bool.eq_iff_iff.mpr
     rw [ψ.truth_iff_mem hsatψ, φ.truth_iff_mem hsatφ]
-  refine ⟨η, PathCond.le_union_left, ?_⟩
-  exact (PathCond.toForm_antitone (PathCond.le_union_right hcompat)).trans (hφ.1 x hx)
+  have hr : α.ReachableWith ψ x := by
+    refine ⟨η, PathCond.le_union_left, ?_⟩
+    exact (PathCond.toForm_antitone (PathCond.le_union_right hcompat)).trans (hφ.1 x hx)
+  refine hψ.2.2 hnx htest ?_ hr
+  · apply (not_reachableWith_of_form_le_stuck hψ.2.1).mt
+    exact not_not.mpr hr
 
 lemma branches_not_mutually_sat {α : Lpofin (Label act test)} {φ ψ : PathCond α}
     (hφ : φ ∈ α.branches) (hψ : ψ ∈ α.branches) (hneq : φ ≠ ψ) :
